working on symbolic evaluation tactics... somewhat working.

src/SepTac.v
@@ -9,13 +9,14 @@ Require Expr SepExpr.
 Module SEP := SepExpr.SepExpr BedrockHeap ST.
 
 Definition bedrock_types : list Expr.type :=
-  (** TODO: I think that we want a comparable W **)
   {| Expr.Impl := W 
    ; Expr.Eq := fun x y => 
      match weq x y with
        | left pf => Some pf 
        | _ => None 
-     end |} :: SEP.defaultType (settings * state)%type :: nil.
+     end |}
+  :: SEP.defaultType (settings * state)%type
+  :: SEP.defaultType label :: nil.
 
 Lemma ApplyCancelSep : forall types funcs sfuncs (l r : SEP.sexpr (bedrock_types ++ types) (Expr.tvType O) (Expr.tvType 1)),
   (forall cs,
@@ -64,3 +65,1043 @@ Ltac reflect_goal isConst Ts :=
           apply (@Himp_to_SEP_himp _ funcs sfuncs L R)
       end
   end.
+
+(** Symbolic Evaluation **)
+Require SymEval.
+
+Module PLUGIN := SymEval.EvaluatorPlugin BedrockHeap ST.
+
+Module BedrockEvaluator.
+  Require Import SepExpr SymEval.
+  Require Import Expr.
+
+  Module SEP := PLUGIN.SEP.
+
+  Section typed.
+    Variable types : list type.
+   
+  (** These the reflected version of the IL, it essentially 
+   ** replaces all uses of W with expr types so that the value
+   ** can be inspected.
+   **)
+  Inductive sym_loc :=
+  | SymReg : reg -> sym_loc
+  | SymImm : expr types -> sym_loc
+  | SymIndir : reg -> expr types -> sym_loc.
+
+  (* Valid targets of assignments *)
+  Inductive sym_lvalue :=
+  | SymLvReg : reg -> sym_lvalue
+  | SymLvMem : sym_loc -> sym_lvalue.
+  
+  (* Operands *)
+  Inductive sym_rvalue :=
+  | SymRvLval : sym_lvalue -> sym_rvalue
+  | SymRvImm : expr types -> sym_rvalue
+  | SymRvLabel : label -> sym_rvalue.
+
+  (* Non-control-flow instructions *)
+  Inductive sym_instr :=
+  | SymAssign : sym_lvalue -> sym_rvalue -> sym_instr
+  | SymBinop : sym_lvalue -> sym_rvalue -> binop -> sym_rvalue -> sym_instr.
+
+  Inductive sym_jmp :=
+    SymUncond : sym_rvalue -> sym_jmp
+  | SymCond : sym_rvalue -> test -> sym_rvalue -> label -> label -> sym_jmp.
+
+  End typed.
+
+  Section typed_ext.
+    Variable types' : list type.
+    Definition types := bedrock_types ++ types'.
+    Definition pcT := tvType 0.
+    Definition stT := tvType 1.
+    Definition lblT := tvType 1.
+  
+  (** Symbolic registers **)
+  Definition SymRegType : Type :=
+    (expr types * expr types * expr types)%type.
+
+  Definition sym_getReg (r : reg) (sr : SymRegType) : expr types :=
+    match r with
+      | Sp => fst (fst sr)
+      | Rp => snd (fst sr)
+      | Rv => snd sr
+    end.
+
+  Definition sym_setReg (r : reg) (v : expr types) (sr : SymRegType) : SymRegType :=
+    match r with
+      | Sp => (v, snd (fst sr), snd sr)
+      | Rp => (fst (fst sr), v, snd sr)
+      | Rv => (fst sr, v)
+    end.
+
+  Variable funcs : functions types.
+  Variable fPlus fMinus fTimes : expr types -> expr types -> expr types.
+  Variable sfuncs : list (SEP.ssignature types pcT stT).
+
+  Variable known : list nat.
+  Definition smem_read stn := SepIL.ST.HT.smem_get_word (IL.implode stn).
+  Definition smem_write stn := SepIL.ST.HT.smem_set_word (IL.explode stn).
+
+  Variable word_evals : hlist (fun n : nat => match nth_error sfuncs n with
+                                                | None => Empty_set 
+                                                | Some ss => @PLUGIN.SymEval types stT pcT pcT pcT smem_read smem_write funcs ss
+                                              end) known.
+
+  Definition symeval_read_word (hyps : list (expr types)) (p : expr types) 
+    (s : SEP.SHeap types pcT stT)
+    : option (expr types) :=
+    let hyps := hyps ++ SepExpr.pures s in
+    let reader ss seb args :=
+      PLUGIN.sym_read seb hyps args p
+    in
+    SymEval.fold_known _ _ reader (SepExpr.impures s) word_evals.
+
+  Definition symeval_write_word (hyps : list (expr types)) (p v : expr types) 
+    (s : SEP.SHeap types pcT stT)
+    : option (SEP.SHeap types pcT stT) :=
+    let hyps := hyps ++ SepExpr.pures s in
+    let writer _ seb args := 
+      PLUGIN.sym_write seb hyps args p v
+    in
+    match SymEval.fold_known_update _ _ writer (SepExpr.impures s) word_evals with
+      | None => None
+      | Some i' => Some {| SepExpr.impures := i' ; SepExpr.pures := SepExpr.pures s ; SepExpr.other := SepExpr.other s |}
+    end.
+
+  Lemma symeval_write_word_correct' : forall hyps pe ve s s',
+    symeval_write_word hyps pe ve s = Some s' ->
+    forall cs stn uvars vars m v,
+      AllProvable funcs uvars vars hyps ->
+      exprD funcs uvars vars ve pcT = Some v ->
+      (exists sm, 
+           SepIL.ST.satisfies cs (SEP.sexprD funcs sfuncs uvars vars (SEP.sheapD s)) stn sm
+        /\ SepIL.ST.HT.satisfies sm m) ->
+      match exprD funcs uvars vars pe pcT with
+        | Some p =>
+          exists m', 
+                mem_set_word _ _  footprint_w SepIL.BedrockHeap.mem_set (IL.explode stn) p v m = Some m'
+            /\ exists sm,
+               SepIL.ST.satisfies cs (SEP.sexprD funcs sfuncs uvars vars (SEP.sheapD s')) stn sm
+            /\ SepIL.ST.HT.satisfies sm m'
+        | _ => False
+      end.
+  Proof.
+    unfold symeval_write_word. intros.
+    generalize dependent H.
+    match goal with
+      | [ |- context [ fold_known_update ?A ?B ?C ?D ?E ] ] =>
+        case_eq (fold_known_update A B C D E); intros; try congruence
+    end.
+    eapply fold_known_update_correct in H.
+    do 5 destruct H. destruct H2.
+    intuition. inversion H3; clear H3; subst. 
+        
+    eapply fold_args_update_correct in H6.
+    repeat match goal with
+             | [ H : exists x, _ |- _ ] => destruct H
+           end. intuition; subst.
+    generalize (SEP.sheapD_pures _ _ _ _ _ H4).
+    rewrite SEP.sheapD_pull_impure in H4 by eauto.
+    rewrite SEP.starred_In in H4.
+    rewrite <- SEP.heq_star_assoc in H4. rewrite SEP.heq_star_comm in H4.
+        
+    simpl in *. rewrite H2 in *.
+    intros.
+
+    eapply SepIL.ST.satisfies_star in H4. do 2 destruct H4. intuition.
+
+    eapply PLUGIN.sym_write_correct with (stn := stn) (cs := cs) (m := x2)
+      in H3; eauto.
+
+    2: apply AllProvable_app; eauto.
+    2: simpl in *;
+    match goal with
+      | [ |- context [ applyD ?A ?B ?C ?D ?E ] ] =>
+        destruct (applyD A B C D E); try solve [ intros; intuition | eapply SepIL.ST.satisfies_pure in H4; PropXTac.propxFo ]
+    end.
+
+    destruct (exprD funcs uvars vars pe pcT); eauto.
+
+    repeat match goal with
+             | [ H : context [ match applyD ?A ?B ?C ?D ?E with
+                                 | Some _ => _
+                                 | None => _ 
+                               end ] |- _ ] =>
+               generalize dependent H; case_eq (applyD A B C D E); intros; intuition
+             | [ H : SepIL.ST.satisfies _ (SepIL.ST.inj _) _ _ |- _ ] =>
+               eapply SepIL.ST.satisfies_pure in H; PropXTac.propxFo; instantiate; intuition
+           end.
+    generalize dependent H8. case_eq (smem_write stn t v x2); intros; intuition.
+
+    unfold smem_write in H8.
+    pose (SepIL.ST.HT.join s0 x3).
+
+    destruct (@SepIL.ST.HT.satisfies_set_word x4 m H5 (explode stn) t v (SepIL.ST.HT.join s0 x3)).
+      destruct H7; subst.
+      eapply SepIL.ST.HT.split_set_word in H8; eauto.
+      intuition eauto.
+
+       
+    destruct H12. eexists; split; eauto.
+    eexists; split; [ | eauto ].
+
+    rewrite SEP.sheapD_pull_impure by eapply FM.find_add.
+    rewrite SEP.starred_In. rewrite <- SEP.heq_star_assoc.
+    rewrite SEP.heq_star_comm.
+
+    simpl.
+    eapply SepIL.ST.satisfies_star.
+
+    rewrite H2. simpl in H3. rewrite H3. exists s0.
+    exists x3. rewrite FM.remove_add. intuition.
+
+    eapply SepIL.ST.HT.disjoint_split_join.
+
+    eapply SepIL.ST.HT.split_set_word in H8.
+    2: destruct H7; eauto.
+    intuition eauto.
+  Qed.
+
+  Lemma symeval_read_word_correct' : forall hyps pe ve s,
+    symeval_read_word hyps pe s = Some ve ->
+    forall cs stn uvars vars m,
+      AllProvable funcs uvars vars hyps ->
+      (exists sm, 
+        SepIL.ST.satisfies cs (SEP.sexprD funcs sfuncs uvars vars (SEP.sheapD s)) stn sm
+        /\ SepIL.ST.HT.satisfies sm m) ->
+      match exprD funcs uvars vars pe pcT, exprD funcs uvars vars ve pcT with
+        | Some p , Some v =>
+          mem_get_word _ _  footprint_w SepIL.BedrockHeap.mem_get (IL.implode stn) p m = Some v
+        | _ , _ => False
+      end.
+  Proof.
+    unfold symeval_read_word. intros.
+    eapply fold_known_correct in H.
+    do 5 destruct H. destruct H1.
+    intuition. 
+
+    generalize (SEP.sheapD_pures _ _ _ _ _ H); intros.
+
+    eapply SEP.sheapD_pull_impure 
+      with (funcs := funcs) (sfuncs := sfuncs) (a := uvars) (c := vars) (cs := cs)
+        in H1.
+    apply In_split in H3. destruct H3. destruct H3.
+    subst. 
+    rewrite SEP.starred_In with (x := x3) (ls := x5) (ls' := x6) in H1.
+
+    rewrite <- SEP.heq_star_assoc in H1. rewrite SEP.heq_star_comm in H1.
+    rewrite H1 in H.
+    simpl in H.
+    rewrite H2 in *.
+    eapply SepIL.ST.satisfies_star in H. destruct H. destruct H. intuition.
+    
+    eapply PLUGIN.sym_read_correct 
+      with (uvars := uvars) (vars := vars) (cs := cs) (stn := stn) (m := x2)
+        in H6.
+    2: eapply AllProvable_app; auto.
+    destruct (exprD funcs uvars vars pe pcT); auto.
+    destruct (exprD funcs uvars vars ve pcT); auto.
+
+    eapply SepIL.ST.HT.satisfies_get_word; eauto.
+    eapply SepIL.ST.HT.split_smem_get_word; eauto.
+
+    unfold tvarD. simpl.
+    match goal with 
+      | [ |- context [ applyD ?A ?B ?C ?D ?E ] ] =>
+        destruct (applyD A B C D E)
+    end; auto.
+    eapply SepIL.ST.satisfies_pure in H. PropXTac.propxFo.
+  Qed.
+
+  Require Import EqdepClass. 
+
+  Lemma satisfies_defn : forall cs se stn st,
+    PropX.interp cs (SepIL.SepFormula.sepFormula se (stn, st)) <->
+    (exists sm, 
+         SepIL.ST.satisfies cs se stn sm
+      /\ SepIL.ST.HT.satisfies sm (Mem st)).
+  Proof.
+    rewrite SepIL.SepFormula.sepFormula_eq in *. unfold SepIL.sepFormula_def.
+    intros. destruct st; simpl. clear.
+    split; intros.
+    Focus.
+    eexists; split; eauto.
+      unfold SepIL.ST.HT.satisfies, SepIL.memoryIn.
+      rewrite SepIL.AllWords.memoryIn_eq.
+      generalize (SepIL.fcong (fun width : nat => list (word width)) 32
+          (Logic.eq_sym SepIL.AllWords.allWords_eq)).
+      unfold SepIL.memoryIn_def, SepIL.BedrockHeap.all_addr, mem, W, SepIL.allWords_def in *.
+      generalize dependent (SepIL.AllWords.allWords 32).
+      intros. generalize e. rewrite <- e; clear e.
+      uip_all.
+      clear. induction (pow2 32).
+        compute; trivial.
+
+        split;
+          unfold SepIL.BedrockHeap.mem_get, SepIL.BedrockHeap.mem_acc, ReadByte.
+          destruct (Mem $ n); split; try eexists; reflexivity.
+
+          eassumption.
+
+    Focus.
+(*
+    destruct H. intuition.
+      unfold SepIL.ST.satisfies in *.
+      revert H0. revert H1.
+      unfold SepIL.ST.HT.satisfies, SepIL.memoryIn.
+      rewrite SepIL.AllWords.memoryIn_eq.
+      generalize (SepIL.fcong (fun width : nat => list (word width)) 32
+        (Logic.eq_sym SepIL.AllWords.allWords_eq)).
+      unfold SepIL.hpropB, SepIL.ST.hprop in *.
+      unfold mem, W, SepIL.ST.HT.smem in *.
+      unfold SepIL.BedrockHeap.all_addr in *.
+      revert Mem. revert x. revert se.
+      generalize dependent (SepIL.AllWords.allWords 32).
+      intros. revert H1. generalize dependent x.
+      revert se. rewrite <- e.
+      unfold SepIL.allWords_def.
+      unfold SepIL.memoryIn_def. clear.
+      generalize (pow2 32).
+      unfold SepIL.memoryInUpto, SepIL.BedrockHeap.mem_get, SepIL.BedrockHeap.mem_acc in *.
+      (** TODO: how do I prove this? **)
+*)
+   (* the only way to prove this seems to be by parametricity..., this is problematic *)
+    admit.
+
+  Qed.
+
+  Lemma symeval_read_word_correct : forall hyps pe ve s,
+    symeval_read_word hyps pe s = Some ve ->
+    forall cs stn uvars vars st,
+      AllProvable funcs uvars vars hyps ->
+      PropX.interp cs (SepIL.SepFormula.sepFormula (SEP.sexprD funcs sfuncs uvars vars (SEP.sheapD s)) (stn, st)) ->
+      match exprD funcs uvars vars pe pcT , exprD funcs uvars vars ve pcT with
+        | Some p , Some v =>
+          mem_get_word _ _  footprint_w SepIL.BedrockHeap.mem_get (IL.implode stn) p (Mem st) = Some v
+        | _ , _ => False
+      end.
+  Proof.
+    intros. eapply symeval_read_word_correct' with (cs := cs) (stn := stn) (m := Mem st) in H; eauto.
+    eapply satisfies_defn; auto.
+  Qed.
+     
+  Theorem symeval_write_word_correct : forall hyps pe ve s s',
+    symeval_write_word hyps pe ve s = Some s' ->
+    forall cs stn uvars vars st v,
+      AllProvable funcs uvars vars hyps ->
+      exprD funcs uvars vars ve pcT = Some v ->
+      PropX.interp cs (SepIL.SepFormula.sepFormula (SEP.sexprD funcs sfuncs uvars vars (SEP.sheapD s)) (stn, st)) ->
+      match exprD funcs uvars vars pe pcT with
+        | Some p =>
+          match mem_set_word _ _ footprint_w SepIL.BedrockHeap.mem_set (IL.explode stn) p v (Mem st) with
+            | Some m' => 
+              PropX.interp cs 
+                (SepIL.SepFormula.sepFormula (SEP.sexprD funcs sfuncs uvars vars (SEP.sheapD s')) 
+                (stn, {| Regs := Regs st ; Mem := m' |}))
+            | None => False
+          end
+        | _ => False
+      end.
+  Proof.
+    intros. eapply symeval_write_word_correct' with (cs := cs) (stn := stn) (m := Mem st) in H; eauto.
+    2: eapply satisfies_defn; eauto.
+    destruct (exprD funcs uvars vars pe pcT); intuition. destruct H.
+    intuition. rewrite H3.
+    eapply satisfies_defn; eauto.
+  Qed.
+
+  (** Symbolic State **)
+  Record SymState : Type :=
+  { SymMem  : SEP.SHeap types pcT stT
+  ; SymRegs : SymRegType
+  }.
+
+  (** This has to be connected to the type of the intermediate representation **)
+  Definition tvWord := tvType 0.
+
+  Definition sym_evalLoc (lv : sym_loc types) (ss : SymState) : expr types :=
+    match lv with
+      | SymReg r => sym_getReg r (SymRegs ss)
+      | SymImm l => l
+      | SymIndir r w => fPlus (sym_getReg r (SymRegs ss)) w
+    end.
+
+  Definition sym_evalLval (lv : sym_lvalue types) (val : expr types) (ss : SymState) : option SymState :=
+    match lv with
+        | SymLvReg r =>
+          Some {| SymMem := SymMem ss ; SymRegs := sym_setReg r val (SymRegs ss) |}
+        | SymLvMem l => 
+          let l := sym_evalLoc l ss in
+          match symeval_write_word (pures (SymMem ss)) l val (SymMem ss) with
+            | Some m =>
+              Some {| SymMem := m ; SymRegs := SymRegs ss |}
+            | None => None
+          end
+    end.
+
+  Definition sym_evalRval (rv : sym_rvalue types) (ss : SymState) : option (expr types) :=
+    match rv with
+      | SymRvLval (SymLvReg r) =>
+        Some (sym_getReg r (SymRegs ss))
+      | SymRvLval (SymLvMem l) =>
+        let l := sym_evalLoc l ss in
+        symeval_read_word (pures (SymMem ss)) l (SymMem ss)
+      | SymRvImm w => Some w 
+      | SymRvLabel l => None (* Labels stn l *)
+    end.
+
+  Definition sym_evalInstr (i : sym_instr types) (ss : SymState) : option SymState :=
+    match i with 
+      | SymAssign lv rv =>
+        match sym_evalRval rv ss with
+          | None => None
+          | Some rv => sym_evalLval lv rv ss
+        end
+      | SymBinop lv l o r =>
+        match sym_evalRval l ss , sym_evalRval r ss with
+          | Some l , Some r => 
+            let v :=
+              match o with
+                | Plus  => fPlus
+                | Minus => fMinus
+                | Times => fTimes                  
+              end l r
+            in
+            sym_evalLval lv v ss
+          | _ , _ => None
+        end
+    end.
+
+  Fixpoint sym_evalInstrs (is : list (sym_instr types)) (ss : SymState) : option SymState :=
+    match is with
+      | nil => Some ss
+      | i :: is => match sym_evalInstr i ss with
+                     | None => None
+                     | Some ss => sym_evalInstrs is ss
+                   end
+    end.
+
+  Variable resolveCond : forall (hyps : list (expr types)) (l : expr types) (tst : test) (r : expr types), option bool.
+
+  Fixpoint sym_evalJmp (j : sym_jmp types) (ss : SymState) : option (SymState * list (list (expr types) * expr types)) :=
+    match j with
+      | SymUncond rv => match sym_evalRval rv ss with
+                          | None => None
+                          | Some v => Some (ss, (nil, v) :: nil)
+                        end
+      | SymCond rvl tst rvr l1 l2 =>
+        match sym_evalRval rvl ss , sym_evalRval rvr ss with
+          | Some l, Some r =>
+            match resolveCond (pures (SymMem ss)) l tst r with
+              | Some true => None (* Some (ss, (nil, @Expr.Const types pcT l1)) *)
+              | Some false => None (* Some (ss, (nil, @Expr.Const types pcT l1)) *)
+              | None => None (* Some (ss, (nil, @Expr.Const types pcT l1)) *)
+            end
+          | _ , _ => None
+        end
+    end.
+
+  Hypothesis fPlus_correct : forall l r uvars vars, 
+    match exprD funcs uvars vars l tvWord , exprD funcs uvars vars r tvWord with
+      | Some lv , Some rv =>
+        exprD funcs uvars vars (fPlus l r) tvWord = Some (wplus lv rv)
+      | _ , _ => True
+    end.
+  Hypothesis fMinus_correct : forall l r uvars vars, 
+    match exprD funcs uvars vars l tvWord , exprD funcs uvars vars r tvWord with
+      | Some lv , Some rv =>
+        exprD funcs uvars vars (fMinus l r) tvWord = Some (wminus lv rv)
+      | _ , _ => True
+    end.
+  Hypothesis fTimes_correct : forall l r uvars vars, 
+    match exprD funcs uvars vars l tvWord , exprD funcs uvars vars r tvWord with
+      | Some lv , Some rv =>
+        exprD funcs uvars vars (fTimes l r) tvWord = Some (wmult lv rv)
+      | _ , _ => True
+    end.
+
+  (* Denotation functions *)
+  Section sym_denote.
+    Variable uvars vars : env types.
+
+    Definition sym_regsD (rs : SymRegType) : option regs :=
+      match rs with
+        | (sp, rp, rv) =>
+          match 
+            exprD funcs uvars vars sp tvWord ,
+            exprD funcs uvars vars rp tvWord ,
+            exprD funcs uvars vars rv tvWord 
+            with
+            | Some sp , Some rp , Some rv =>
+                Some (fun r => 
+                  match r with
+                    | Sp => sp
+                    | Rp => rp
+                    | Rv => rv
+                  end)
+            | _ , _ , _ => None
+          end
+      end.    
+
+    Definition sym_locD (s : sym_loc types) : option loc :=
+      match s with
+        | SymReg r => Some (Reg r)
+        | SymImm e =>
+          match exprD funcs uvars vars e tvWord with
+            | Some e => Some (Imm e)
+            | None => None
+          end
+        | SymIndir r o =>
+          match exprD funcs uvars vars o tvWord with
+            | Some o => Some (Indir r o)
+            | None => None
+          end
+      end.
+
+    Definition sym_lvalueD (s : sym_lvalue types) : option lvalue :=
+      match s with
+        | SymLvReg r => Some (LvReg r)
+        | SymLvMem l => match sym_locD l with
+                          | Some l => Some (LvMem l)
+                          | None => None
+                        end
+      end.
+
+    Definition sym_rvalueD (r : sym_rvalue types) : option rvalue :=
+      match r with
+        | SymRvLval l => match sym_lvalueD l with
+                           | Some l => Some (RvLval l)
+                           | None => None
+                         end
+        | SymRvImm e => match exprD funcs uvars vars e tvWord with
+                          | Some l => Some (RvImm l)
+                          | None => None
+                        end
+        | SymRvLabel l => Some (RvLabel l)
+      end.
+
+    Definition sym_instrD (i : sym_instr types) : option instr :=
+      match i with
+        | SymAssign l r =>
+          match sym_lvalueD l , sym_rvalueD r with
+            | Some l , Some r => Some (Assign l r)
+            | _ , _ => None
+          end
+        | SymBinop lhs l o r =>
+          match sym_lvalueD lhs , sym_rvalueD l , sym_rvalueD r with
+            | Some lhs , Some l , Some r => Some (Binop lhs l o r)
+            | _ , _ , _ => None
+          end
+      end.
+
+    Fixpoint sym_instrsD (is : list (sym_instr types)) : option (list instr) :=
+      match is with
+        | nil => Some nil
+        | i :: is => 
+          match sym_instrD i , sym_instrsD is with
+            | Some i , Some is => Some (i :: is)
+            | _ , _ => None
+          end
+      end.
+
+    Definition regsD (r : regs) (sr : SymRegType) : Prop :=
+      let '(sp, rp, rv) := sr in
+         exprD funcs uvars vars sp tvWord = Some (r Sp)
+      /\ exprD funcs uvars vars rp tvWord = Some (r Rp)
+      /\ exprD funcs uvars vars rv tvWord = Some (r Rv).
+
+    Require Import PropX.
+
+    Definition stateD cs (stn : IL.settings) (s : state) (ss : SymState) : Prop :=
+      PropX.interp cs 
+        ([| regsD (Regs s) (SymRegs ss) |] /\ 
+         SepIL.SepFormula.sepFormula (SEP.sexprD funcs sfuncs uvars vars (SEP.sheapD (SymMem ss))) (stn, s))%PropX.
+
+  End sym_denote.
+
+  Ltac sound_simp :=
+    repeat match goal with 
+             | [ H : match ?X with
+                       | (_, _) => _
+                     end |- _ ] =>
+             destruct X
+             | [ H : match ?X with
+                       | Some _ => _
+                       | None => _
+                     end |- _ ] =>
+             generalize dependent H; case_eq X; intros; try congruence; simpl in *
+             | [ H : match ?X with
+                       | Some _ => _
+                       | None => _
+                     end = _ |- _ ] =>
+             generalize dependent H; case_eq X; intros; try congruence; simpl in *
+             | [ H : match ?X with
+                       | SymLvReg _ => _
+                       | SymLvMem _ => _
+                     end = _ |- _ ] =>
+             generalize dependent H; case_eq X; intros; try congruence; simpl in *
+             | [ H : Some _ = Some _ |- _ ] => inversion H; clear H; subst; simpl in *
+             | [ |- exists x, _ /\ Some _ = Some x ] =>
+               eexists; split; [ | reflexivity ]
+           end; simpl.
+
+  Lemma sym_getReg_sound : forall stn specs uvars vars r ss s,
+    stateD uvars vars specs stn s ss ->
+    exprD funcs uvars vars (sym_getReg r (SymRegs ss)) tvWord = Some (Regs s r).
+  Proof.
+    destruct ss; simpl in *; intros.
+    unfold stateD, regsD in *.
+    PropXTac.propxFo.
+    sound_simp. intuition. destruct r; simpl.
+    rewrite H; auto.
+    rewrite H0; auto.
+    rewrite H3; auto.
+  Qed.
+
+  Lemma sym_loc_sound : forall uvars vars l lD,
+    sym_locD uvars vars l = Some lD ->
+    forall specs stn s ss, 
+      stateD uvars vars specs stn s ss ->
+      forall a,
+        sym_evalLoc l ss = a ->
+        exprD funcs uvars vars a tvWord = Some (evalLoc s lD).
+  Proof.
+    destruct l; intros; subst; simpl in *; sound_simp; eauto.
+    erewrite sym_getReg_sound by eauto. reflexivity.
+    generalize (fPlus_correct (sym_getReg r (SymRegs ss)) e uvars vars).
+    rewrite H.
+    erewrite sym_getReg_sound by eauto. auto.
+  Qed.    
+
+  Lemma pures_implied : forall uvars vars0 specs stn s0 ss,
+    PropX.interp specs
+    (SepIL.SepFormula.sepFormula
+      (SEP.sexprD funcs sfuncs uvars vars0 (SEP.sheapD (SymMem ss)))
+      (stn, s0)) ->
+    AllProvable funcs uvars vars0 (pures (SymMem ss)).
+  Proof.
+    intros.
+    rewrite SepIL.SepFormula.sepFormula_eq in *.
+    unfold SepIL.sepFormula_def in *. simpl in *.
+    generalize SEP.sheapD_pures.
+    unfold SepIL.ST.satisfies.
+    intro. eapply (@H0 _ funcs _ _ sfuncs stn (SepIL.memoryIn (Mem s0)) specs
+    uvars vars0).
+    PropXTac.propxFo.
+  Qed.
+  
+  Local Hint Resolve pures_implied.
+     
+  Lemma stateD_pures : forall uvars vars0 specs stn s0 ss,
+    stateD uvars vars0 specs stn s0 ss ->
+    AllProvable funcs uvars vars0 (pures (SymMem ss)).
+  Proof.
+    intros. unfold stateD in *.
+    PropXTac.propxFo. eauto.
+  Qed.
+
+  Local Hint Resolve stateD_pures.
+
+  Lemma sym_lvalue_sound : forall uvars vars0 l lD,
+    sym_lvalueD uvars vars0 l = Some lD ->
+    forall specs stn s ss, 
+      stateD uvars vars0 specs stn s ss ->
+      forall a aD ss',
+        exprD funcs uvars vars0 a tvWord = Some aD ->
+        sym_evalLval l a ss = Some ss' ->
+        exists s' , 
+          evalLvalue stn s lD aD = Some s'
+          /\ stateD uvars vars0 specs stn s' ss'.
+  Proof.
+(*
+    destruct l; simpl; intros; try congruence.
+    inversion H; clear H; subst.
+    inversion H2; clear H2; subst.
+    simpl; eexists; split; [ reflexivity | ].
+    unfold stateD, regsD in *. PropXTac.propxFo.
+    destruct (SymRegs ss). destruct p.
+    destruct r; simpl in *; intuition.
+    rewrite SepIL.SepFormula.sepFormula_eq in *.
+    unfold SepIL.sepFormula_def in *. simpl in *. auto.
+    
+    repeat match goal with
+             | [ H : match ?X with 
+                       | Some _ => _
+                       | None => _
+                     end = Some _ |- _ ] => 
+               revert H; case_eq X; intros; try congruence
+             | [ H : Some _ = Some _ |- _ ] => 
+               inversion H; clear H; subst
+           end.
+    eapply sym_loc_sound in H; eauto.    
+    unfold stateD in H0. PropXTac.propxFo.
+    eapply symeval_write_word_correct in H2; eauto;
+      unfold stateD in *; PropXTac.propxFo.
+
+    Focus.
+    unfold pcT, tvWord in *. rewrite H in H2.
+    sound_simp. unfold WriteWord, SepIL.BedrockHeap.mem_set in *.
+    rewrite H0. eexists; split; eauto.
+    unfold stateD. 
+    rewrite SepIL.SepFormula.sepFormula_eq in *. simpl in *.
+    PropXTac.propxFo. intuition.
+*)
+  Admitted.
+
+  Lemma sym_rvalue_sound : forall uvars vars0 r rD,
+    sym_rvalueD uvars vars0 r = Some rD ->
+    forall specs stn s ss, 
+      stateD uvars vars0 specs stn s ss ->
+      forall rv,
+        sym_evalRval r ss = Some rv ->
+        exists rvD ,
+          exprD funcs uvars vars0 rv tvWord = Some rvD /\
+          evalRvalue stn s rD = Some rvD.
+  Proof.
+    destruct r; simpl; intros.
+      sound_simp. erewrite sym_getReg_sound; eauto.
+      
+      Focus.
+      eapply symeval_read_word_correct with (vars := vars0) (uvars := uvars) 
+        (cs := specs) (stn := stn) (st := s0) in H3; eauto.
+        erewrite sym_loc_sound in H3 by eauto.
+        unfold ReadWord, SepIL.BedrockHeap.mem_get in *.
+        unfold pcT, tvWord in *.
+        destruct (exprD funcs uvars vars0 rv (tvType 0)); intuition.
+        eexists; intuition eauto.
+        unfold stateD in *. PropXTac.propxFo.
+
+      Focus.
+      sound_simp; auto.
+
+      Focus.
+      congruence.
+  Qed.
+
+  Lemma sym_binops : forall uvars vars0 b e e0 x x0,
+    exprD funcs uvars vars0 e tvWord = Some x ->
+    exprD funcs uvars vars0 e0 tvWord = Some x0 ->
+    exprD funcs uvars vars0
+    (match b with
+       | Plus => fPlus
+       | Minus => fMinus
+       | Times => fTimes
+     end e e0) tvWord = Some (evalBinop b x x0).
+  Proof.
+    destruct b; simpl; intros.
+      generalize (fPlus_correct e e0 uvars vars0); rewrite H; rewrite H0; auto.
+      generalize (fMinus_correct e e0 uvars vars0); rewrite H; rewrite H0; auto.
+      generalize (fTimes_correct e e0 uvars vars0); rewrite H; rewrite H0; auto.
+  Qed.
+    
+  Theorem sym_evalInstr_sound : forall i iD uvars vars, 
+    sym_instrD uvars vars i = Some iD ->
+    forall stn ss ss',
+    sym_evalInstr i ss = Some ss' ->
+    forall specs s,
+    stateD uvars vars specs stn s ss ->
+    exists s',
+    evalInstr stn s iD = Some s' /\ stateD uvars vars specs stn s' ss'.
+  Proof.
+    destruct i; simpl; intros iD uvars vars0.
+
+      intros; sound_simp; try congruence.
+      eapply sym_rvalue_sound in H3; eauto.
+      destruct H3. intuition.
+      eapply sym_lvalue_sound in H2; eauto.
+      destruct H2; intuition.
+      rewrite H5. eauto.
+
+      intros; sound_simp; try congruence.
+      eapply sym_rvalue_sound in H0; eauto.
+      eapply sym_rvalue_sound in H2; eauto.
+      destruct H0; destruct H2; intuition.
+      rewrite H7. rewrite H8.
+      
+      eapply sym_lvalue_sound in H3; eauto.
+      eapply sym_binops; eauto.
+  Qed.
+
+  Theorem sym_evalInstrs_sound : forall i iD uvars vars, 
+    sym_instrsD uvars vars i = Some iD ->
+    forall stn ss ss',
+    sym_evalInstrs i ss = Some ss' ->
+    forall specs s,
+    stateD uvars vars specs stn s ss ->
+    exists s',
+    evalInstrs stn s iD = Some s' /\ stateD uvars vars specs stn s' ss'.
+  Proof.
+    induction i; simpl; intros.
+      inversion H0; clear H0; inversion H; clear H; subst; simpl. eauto.
+
+      sound_simp.
+      eapply sym_evalInstr_sound in H; eauto.
+      destruct H; intuition.
+      rewrite H4.
+      eauto.
+  Qed.
+
+  (** TODO: This isn't done **)
+  Definition reflect_regs sp rv rp : SymRegType :=
+    (@Expr.Const types (tvType 0) sp,
+     @Expr.Const types (tvType 0) rv,
+     @Expr.Const types (tvType 0) rp).
+
+  Require Import PropX.
+
+  Theorem sym_evalInstrs_apply : forall uvars vars cs instrs stn st st', 
+    evalInstrs stn st instrs = Some st' ->
+    forall sp rv rp sh,
+      PropX.interp cs (SepIL.SepFormula.sepFormula (SEP.sexprD funcs sfuncs uvars vars sh) (stn, st)%PropX) ->
+      exprD funcs uvars vars sp tvWord = Some (Regs st Sp) ->
+      exprD funcs uvars vars rv tvWord = Some (Regs st Rv) ->
+      exprD funcs uvars vars rp tvWord = Some (Regs st Rp) ->
+    forall vars' hashed,
+      SEP.hash sh = (vars' , hashed) ->
+      forall sym_instrs ss',
+      sym_evalInstrs sym_instrs 
+        {| SymRegs := (sp, rp, rv) ;
+           SymMem  := hashed |} = Some ss' ->
+      sym_instrsD uvars vars sym_instrs = Some instrs -> (** TODO: what do I do with vars'? **)
+      stateD uvars vars cs stn st' ss'.
+  Proof.
+    intros. eapply sym_evalInstrs_sound with (specs := cs) (uvars := uvars) (vars := vars) (stn := stn) (s := st) in H5; eauto.
+    Focus 2.
+      unfold stateD in *; simpl in *.
+      PropXTac.propxFo. admit.
+    
+      destruct H5. intuition. rewrite H in H7. inversion H7; clear H7; subst; auto.
+  Qed.
+
+  End typed_ext.
+
+  (* Reflect the instructions *)
+  Ltac collectTypes_loc l Ts :=
+    match l with
+      | Reg _ => Ts
+      | Imm ?i => SEP.collectTypes_expr i Ts
+      | Indir _ ?i => SEP.collectTypes_expr i Ts
+    end.
+  Ltac reflect_loc isConst l types funcs uvars vars k :=
+    match l with
+      | Reg ?r => constr:(@SymReg types r)
+      | Imm ?i =>
+        SEP.reflect_expr isConst i types funcs uvars vars ltac:(fun funcs i =>
+          let l := constr:(@SymImm types i) in k funcs l)
+      | Indir ?r ?i =>
+        SEP.reflect_expr isConst i types funcs uvars vars ltac:(fun funcs i =>
+          let l := constr:(@SymIndir types r i) in k funcs l)
+    end.
+
+  Ltac collectTypes_lvalue l Ts :=
+    match l with
+      | LvReg _ => Ts
+      | LvMem ?l => collectTypes_loc l Ts
+    end.
+  Ltac reflect_lvalue isConst l types funcs uvars vars k :=
+    match l with
+      | LvReg ?r => let l := constr:(@SymLvReg types r) in k funcs l 
+      | LvMem ?l => 
+        reflect_loc isConst l types funcs uvars vars ltac:(fun funcs l =>
+          let l := constr:(@SymLvMem types l) in k funcs l)
+    end.
+
+  Ltac collectTypes_rvalue r Ts :=
+    match r with
+      | RvLval ?l => collectTypes_lvalue l Ts
+      | RvImm ?i => SEP.collectTypes_expr i Ts
+      | RvLabel _ => let l := constr:(label:Type) in Reflect.cons_uniq l Ts
+    end.
+  Ltac reflect_rvalue isConst r types funcs uvars vars k :=
+    match r with
+      | RvLval ?l =>
+        reflect_lvalue isConst l types funcs uvars vars ltac:(fun funcs l =>
+          let l := constr:(@SymRvLval types l) in k funcs l)
+      | RvImm ?i =>
+        (** TODO: something is wrong with this call! **)
+        idtac "found imm" i types funcs ;
+        SEP.reflect_expr isConst i types funcs uvars vars ltac:(fun funcs i =>
+          idtac "got back ";
+          let l := constr:(@SymRvImm types r i) in k funcs l)
+      | RvLabel ?l => 
+        let r := constr:(@SymRvLabel types l) in k funcs r
+    end.
+
+  Ltac collectTypes_instr i Ts :=
+    match i with
+      | Assign ?l ?r =>
+        let Ts := collectTypes_lvalue l Ts in
+        collectTypes_rvalue r Ts
+      | Binop ?l ?r1 _ ?r2 =>
+        let Ts := collectTypes_lvalue l Ts in
+        let Ts := collectTypes_rvalue r1 Ts in
+        collectTypes_rvalue r2 Ts
+    end.
+  Ltac reflect_instr isConst i types funcs uvars vars k :=
+    match i with
+      | Assign ?l ?r =>
+        idtac "1" ;
+        reflect_lvalue isConst l types funcs uvars vars ltac:(fun funcs l =>
+          idtac "2";
+        reflect_rvalue isConst r types funcs uvars vars ltac:(fun funcs r =>
+          idtac "3";
+          let res := constr:(@SymAssign types l r) in k funcs res))
+      | Binop ?l ?r1 ?o ?r2 =>
+        reflect_lvalue isConst l types funcs uvars vars ltac:(fun funcs l =>
+        reflect_rvalue isConst r1 types funcs uvars vars ltac:(fun funcs r1 =>
+        reflect_rvalue isConst r2 types funcs uvars vars ltac:(fun funcs r2 =>
+          let res := constr:(@SymBinop types l r1 o r2) in k funcs res)))
+    end.
+
+  Ltac collectTypes_instrs is Ts :=
+    match is with
+      | nil => Ts
+      | ?i :: ?is => 
+        let Ts := collectTypes_instr i Ts in
+        collectTypes_instrs is Ts
+    end.
+  Ltac reflect_instrs isConst is types funcs uvars vars k :=
+    match is with
+      | nil => 
+        idtac "got to here" ;
+        let is := constr:(@nil (sym_instr types)) in k funcs is
+      | ?i :: ?is =>
+        idtac "here";
+        reflect_instr isConst i types funcs uvars vars ltac:(fun funcs i =>
+          idtac "kk" ;
+        reflect_instrs isConst is types funcs uvars vars ltac:(fun funcs is =>
+          let res := constr:(i :: is) in k funcs res))
+    end.
+
+  Ltac isConst e :=
+    match e with
+      | 0 => true
+      | S ?e => isConst e
+      | true => true
+      | false => false
+      | Regs _ _ => true
+      | _ => false
+    end.
+
+  Definition bedrock_funcs types' : list (signature (types types')).
+  refine ({| Domain := tvWord :: tvWord :: nil
+           ; Range := tvWord
+           ; Denotation := _ |} ::
+          {| Domain := tvWord :: tvWord :: nil
+           ; Range := tvWord
+           ; Denotation := _ |} ::
+          {| Domain := tvWord :: tvWord :: nil
+           ; Range := tvWord
+           ; Denotation := _ |} :: nil).
+  refine (@wplus 32).
+  refine (@wminus 32).
+  refine (@wmult 32).
+  Defined.  
+
+  Definition fPlus types' (l r : expr (types types')) : expr (types types') :=
+    Expr.Func 0 (l :: r :: nil).
+  Definition fMinus types' (l r : expr (types types')) : expr (types types') :=
+    Expr.Func 1 (l :: r :: nil).
+  Definition fMult types' (l r : expr (types types')) : expr (types types') :=
+    Expr.Func 2 (l :: r :: nil).
+
+  Theorem fPlus_correct types' funcs' : forall l r uvars vars, 
+    match exprD (bedrock_funcs types' ++ funcs') uvars vars l tvWord , exprD (bedrock_funcs types' ++ funcs') uvars vars r tvWord with
+      | Some lv , Some rv =>
+        exprD (bedrock_funcs types' ++ funcs') uvars vars (fPlus _ l r) tvWord = Some (wplus lv rv)
+      | _ , _ => True
+    end.
+  Proof.
+    intros. simpl.
+    repeat match goal with
+             | [ |- match ?X with
+                      | Some _ => _
+                      | None => _
+                    end ] => destruct X
+           end; auto.
+  Qed.
+  Theorem fMinus_correct types' funcs' : forall l r uvars vars, 
+    match exprD (bedrock_funcs types' ++ funcs') uvars vars l tvWord , exprD (bedrock_funcs types' ++ funcs') uvars vars r tvWord with
+      | Some lv , Some rv =>
+        exprD (bedrock_funcs types' ++ funcs') uvars vars (fMinus _ l r) tvWord = Some (wminus lv rv)
+      | _ , _ => True
+    end.
+  Proof.
+    intros. simpl.
+    repeat match goal with
+             | [ |- match ?X with
+                      | Some _ => _
+                      | None => _
+                    end ] => destruct X
+           end; auto.
+  Qed.
+  Theorem fMult_correct types' funcs' : forall l r uvars vars, 
+    match exprD (bedrock_funcs types' ++ funcs') uvars vars l tvWord , exprD (bedrock_funcs types' ++ funcs') uvars vars r tvWord with
+      | Some lv , Some rv =>
+        exprD (bedrock_funcs types' ++ funcs') uvars vars (fMult _ l r) tvWord = Some (wmult lv rv)
+      | _ , _ => True
+    end.
+  Proof.
+    intros. simpl.
+    repeat match goal with
+             | [ |- match ?X with
+                      | Some _ => _
+                      | None => _
+                    end ] => destruct X
+           end; auto.
+  Qed.
+
+  Ltac find_reg st r :=
+    match goal with
+      | [ H : Regs st r = ?x |- _ ] => x
+      | _ => constr:((Regs st r, @refl_equal (option W) (Some (Regs st r))))
+    end.
+
+  Goal forall cs stn st st' SF,
+    PropX.interp cs (SepIL.SepFormula.sepFormula SF (stn, st)) ->
+    evalInstrs stn st (Assign Rp Sp (*(RvImm (natToW 0)) *) :: nil) = Some st' ->
+    True.
+  Proof.
+    intros.
+    match goal with
+      | [ H : evalInstrs ?stn ?st ?is = _ 
+        , H' : PropX.interp ?cs (SepIL.SepFormula.sepFormula ?SF (?stn, ?st)) |- _ ] =>
+        match find_reg st Rp with
+          | (?rp_v, ?rp_pf) =>
+            match find_reg st Sp with
+              | (?sp_v, ?sp_pf) =>
+                match find_reg st Rv with
+                  | (?rv_v, ?rv_pf) => 
+        let regs := constr:((rp_v, (sp_v, (rv_v, tt)))) in
+        let Ts := constr:(@nil Type) in
+        let Ts := collectTypes_instrs is Ts in
+        let Ts := SEP.collectAllTypes_expr isConst Ts regs in
+        let Ts := SEP.collectAllTypes_sexpr isConst Ts (SF :: nil) in
+        let types := eval unfold bedrock_types in bedrock_types in
+        let types := SEP.extend_all_types Ts types in
+        let funcs := constr:(@nil (@signature types)) in
+        let sfuncs := constr:(@nil (@SEP.ssignature types pcT stT)) in
+        let uvars := eval simpl in (@nil _ : env types) in
+        let vars := eval simpl in (@nil _ : env types) in
+        reflect_instrs ltac:(isConst) is types funcs uvars vars ltac:(fun funcs sis =>
+        SEP.reflect_expr ltac:(isConst) rp_v types funcs uvars vars ltac:(fun funcs rp_v =>
+        SEP.reflect_expr ltac:(isConst) sp_v types funcs uvars vars ltac:(fun funcs sp_v =>
+        SEP.reflect_expr ltac:(isConst) rv_v types funcs uvars vars ltac:(fun funcs rv_v =>
+        SEP.reflect_sexpr ltac:(isConst) SF types funcs pcT stT sfuncs uvars vars ltac:(fun funcs sfuncs SF =>
+          match types with
+            | _ :: _ :: _ :: ?X =>
+              generalize (@sym_evalInstrs_apply X (bedrock_funcs X) (fPlus _) (fMinus _) (fMult _) sfuncs nil HNil
+                (fPlus_correct _ _) (fMinus_correct _ _) (fMult_correct _ _) uvars vars cs is stn st _ H sp_v rv_v rp_v SF H'
+                sp_pf rv_pf rp_pf _ _ (refl_equal _) sis _ (refl_equal _) (refl_equal _))
+          end)))))
+                end
+            end
+        end
+    end.
+    simpl.
+  Abort.
+
+End BedrockEvaluator.
+
